---
layout: post
title: "Math post"
categories: testing math
---
# A mathematical theorem
<div class="theorem">
For any quadratic equation of the form \(ax^2 + bx + c = 0\), its two solutions are:
$$x = \frac{-b \pm \sqrt{b^2 - 4ac}}{2a}$$
</div>
<div class="proof">
Move the terms to get \(x^2 + \frac{b}{a}x = -\frac{c}{a}\). Using the equation:

$$(x + a)^2 = x^2 + 2ax + a^2$$

, we add \((\frac{b}{2a})^2\) to each side and get:

$$x^2 + 2(\frac{b}{2a})x + (\frac{b}{2a})^2  = (x + \frac{b}{2a})^2
 = -\frac{c}{a} + (\frac{b}{2a})^2
 = \frac{b^2 - 4ac}{4a^2}$$

$$x + \frac{b}{2a}  = \pm\frac{\sqrt{b^2 - 4ac}}{2a}$$

$$x = \frac{-b \pm \sqrt{b^2 - 4ac}}{2a}$$
</div>
